Experiment: universal register invalidation
Because the Allocation pass is a specialized type of static analyzer,
and because the call case makes assertions about sets equations not
constrained by (originally) callee-save registers, an extension of
this pass to a complex, context-sensitive calling convention is not
easily realized.

In order to select one calling convention (the standard ABI with
callee-save registers, which we would like to retain for
intra-compartment crossings) or the other (a secure calling convention
where every register is caller-save and non-argument registers are
moreover invalidated on compartment boundaries, which the proof needs
for the latter case), the static analyzer would need to determine when
a call or a return is changing compartments.

However, the static analyzer operates at the function level and is aware
of the function being analyzed (and its compartment). It does not know
which compartment(s) a call instruction may call into, because this
information is only available dynamically to the semantics based on the
current program state -- barring further restrictions or a more
sophisticated analysis.

For simplicity, we experiment with the extension that conservatively
applies register invalidation to all calls and returns. It remains to
evaluate the performance costs of this approach and the consequences on
the static analysis process itself.

backend/Allocproof.v
@@ -2157,7 +2157,12 @@ Inductive match_stackframes: list RTL.stackframe -> list LTL.stackframe -> signa
         (STEPS: forall v ls1 m,
            Val.lessdef v (Locmap.getpair (map_rpair R (loc_result sg)) ls1) ->
            Val.has_type v (env res) ->
-           agree_callee_save ls ls1 ->
+           (* match Genv.type_of_call ge (call_comp ts) (callee_comp ts (* FIXME *)) with *)
+           (* match Genv.type_of_call ge (comp_of tf) cp with *)
+           (* | Genv.CrossCompartmentCall => agree_callee_save_ext ls ls1 *)
+           (* | _ => agree_callee_save ls ls1 *)
+           (* end -> *)
+           agree_callee_save_ext ls ls1 ->
            exists ls2,
            star LTL.step tge (Block ts tf sp bb ls1 m)
                           E0 (State ts tf sp pc ls2 m)
@@ -2179,15 +2184,15 @@ Definition cp_of_stack (stk: list RTL.stackframe) :=
   | _ => default_compartment
   end.
 
-(* TODO: Relocate *)
-Definition callee_save_loc_ext (l: loc) (callee_sig: signature) : Prop :=
-  match l with
-  | R r => in_mreg r (regs_of_rpair (loc_result callee_sig)) = true
-  | S sl ofs ty => sl <> Outgoing
-  end.
+(* (* TODO: Relocate *) *)
+(* Definition callee_save_loc_ext (l: loc) (callee_sig: signature) : Prop := *)
+(*   match l with *)
+(*   | R r => in_mreg r (regs_of_rpair (loc_result callee_sig)) = true *)
+(*   | S sl ofs ty => sl <> Outgoing *)
+(*   end. *)
 
-Definition agree_callee_save_ext (ls1 ls2: Locmap.t) (callee_sig: signature) : Prop :=
-  forall l, callee_save_loc_ext l callee_sig -> ls1 l = ls2 l.
+(* Definition agree_callee_save_ext (ls1 ls2: Locmap.t) (callee_sig: signature) : Prop := *)
+(*   forall l, callee_save_loc_ext l callee_sig -> ls1 l = ls2 l. *)
 
 Inductive match_states: RTL.state -> LTL.state -> Prop :=
   | match_states_intro:
@@ -2207,7 +2212,7 @@ Inductive match_states: RTL.state -> LTL.state -> Prop :=
         (STACKS: match_stackframes s ts (funsig tf))
         (FUN: transf_fundef f = OK tf)
         (ARGS: Val.lessdef_list args (map (fun p => Locmap.getpair p ls) (loc_arguments (funsig tf))))
-        (AG: agree_callee_save (parent_locset ts) ls)
+        (AG: agree_callee_save_ext (parent_locset ts) ls)
         (MEM: Mem.extends m m')
         (WTARGS: Val.has_type_list args (sig_args (funsig tf))),
       match_states (RTL.Callstate s f args m)
@@ -2216,10 +2221,12 @@ Inductive match_states: RTL.state -> LTL.state -> Prop :=
       forall s res m ts ls m' sg
         (STACKS: match_stackframes s ts sg)
         (RES: Val.lessdef res (Locmap.getpair (map_rpair R (loc_result sg)) ls))
-        (AG: match Genv.type_of_call ge (call_comp ts) (callee_comp ts) with
-             | Genv.CrossCompartmentCall => True
-             | _ => agree_callee_save (parent_locset ts) ls
-             end)
+        (* (AG: match Genv.type_of_call ge (call_comp ts) (callee_comp ts) with *)
+        (*      | Genv.CrossCompartmentCall => agree_callee_save_ext (parent_locset ts) ls *)
+        (*      | _ => agree_callee_save (parent_locset ts) ls *)
+        (*      end) *)
+        (* (AG: agree_callee_save_ext (parent_locset ts) ls) *)
+        (AG: agree_callee_save_ext (parent_locset ts) ls)
         (MEM: Mem.extends m m')
         (WTRES: Val.has_type res (proj_sig_res sg)),
       match_states (RTL.Returnstate s res m)
@@ -2611,7 +2618,7 @@ Proof.
   rewrite <- comp_transf_function; eauto.
   eapply allowed_call_translated; eauto.
   { intros TY_CALL.
-    rewrite TY_CALL.
+    (* rewrite TY_CALL. *)
     assert (X: Genv.type_of_call ge (comp_of f) (Genv.find_comp ge vf) = Genv.CrossCompartmentCall).
     { erewrite find_comp_translated, type_of_call_translated; eauto. rewrite comp_transf_function; eauto. }
     specialize (NO_CROSS_PTR X).
@@ -2686,10 +2693,52 @@ Proof.
     rewrite <- call_regs_param_values in Heqo2.
     rewrite <- call_regs_ext_param_values in Heqo2'.
     (* pose proof (Val.lessdef_list_not_ptr _ _ Heqo2 NO_CROSS_PTR) as H. *)
-    assert (R: map (fun p : rpair loc => Locmap.getpair p (undef_regs destroyed_at_function_entry (call_regs ls1))) (loc_parameters sg) =
-            map (fun p : rpair loc => Locmap.getpair p (call_regs ls1)) (loc_parameters sg)).
-    { (* TODO: try using [Locmap.getpair_exten]
-         TODO: remove the code duplication *)
+    (* assert (R: map (fun p : rpair loc => Locmap.getpair p (undef_regs destroyed_at_function_entry (call_regs ls1))) (loc_parameters sg) = *)
+    (*         map (fun p : rpair loc => Locmap.getpair p (call_regs ls1)) (loc_parameters sg)). *)
+    (* { (* TODO: try using [Locmap.getpair_exten] *)
+    (*      TODO: remove the code duplication *) *)
+    (*   assert (G: forall l rhi rlo, In l (loc_parameters sg) -> l <> One (R R30) /\ l <> Twolong (R R30) rlo /\ l <> Twolong rhi (R R30)). *)
+    (*   { clear. *)
+    (*     unfold loc_parameters. *)
+    (*     destruct l as [[] |]; try congruence. *)
+    (*     - pose proof (loc_arguments_acceptable_stronger sg) as G. *)
+    (*       intros rhi rlo IN. *)
+    (*       eapply in_map_iff in IN as [x [Hx' Hx]]. *)
+    (*       eapply G in Hx. *)
+    (*       destruct x; inv Hx'. *)
+    (*       destruct r0 as [| []]; simpl; try congruence. *)
+    (*       simpl in Hx. destruct Hx. inv H0. split; [| split]; congruence. *)
+    (*       contradiction. *)
+    (*       contradiction. *)
+    (*       split; [| split]; congruence. *)
+    (*     - intros. *)
+    (*       split; [| split]; congruence. *)
+    (*     - pose proof (loc_arguments_acceptable_stronger sg) as G. *)
+    (*       intros rhi' rlo' IN. *)
+    (*       eapply in_map_iff in IN as [x [Hx' Hx]]. *)
+    (*       eapply G in Hx. *)
+    (*       destruct x; inv Hx'. *)
+    (*       destruct rhi0 as [| []]; destruct rlo0 as [| []]; *)
+    (*         destruct Hx as [[] []]; simpl; (split; [| split]); try congruence. *)
+    (*   } *)
+    (*   clear -G. revert G. *)
+    (*   generalize (loc_parameters sg). *)
+    (*   induction l; intros. *)
+    (*   - auto. *)
+    (*   - Local Transparent destroyed_at_function_entry. *)
+    (*     simpl in *. rewrite IHl; auto. *)
+    (*     destruct a; simpl. *)
+    (*     + rewrite Locmap.gso; auto. destruct r as [[] |]; try now simpl. *)
+    (*       now specialize (G (One (R R30)) (R R30) (R R30) (or_introl eq_refl)). *)
+    (*     + rewrite Locmap.gso; auto. rewrite Locmap.gso; auto. *)
+    (*       destruct rlo as [[] |]; try now simpl. *)
+    (*       specialize (G (Twolong rhi (R R30)) (rhi) (R R30) (or_introl eq_refl)) as [? [? ?]]. congruence. *)
+    (*       specialize (G (Twolong rhi rlo) (rhi) (rlo) (or_introl eq_refl)) as [? [? ?]]. *)
+    (*       now destruct rhi; try congruence. } *)
+    assert (R': map (fun p : rpair loc => Locmap.getpair p (undef_regs destroyed_at_function_entry (call_regs_ext ls1 sg))) (loc_parameters sg) =
+                 map (fun p : rpair loc => Locmap.getpair p (call_regs_ext ls1 sg)) (loc_parameters sg)).
+    { (* TODO Same proof as R: refactor *)
+      (* clear R. (* Hides the register constructor *) *)
       assert (G: forall l rhi rlo, In l (loc_parameters sg) -> l <> One (R R30) /\ l <> Twolong (R R30) rlo /\ l <> Twolong rhi (R R30)).
       { clear.
         unfold loc_parameters.
@@ -2728,16 +2777,14 @@ Proof.
           specialize (G (Twolong rhi (R R30)) (rhi) (R R30) (or_introl eq_refl)) as [? [? ?]]. congruence.
           specialize (G (Twolong rhi rlo) (rhi) (rlo) (or_introl eq_refl)) as [? [? ?]].
           now destruct rhi; try congruence. }
-    assert (R': map (fun p : rpair loc => Locmap.getpair p (undef_regs destroyed_at_function_entry (call_regs_ext ls1 sg))) (loc_parameters sg) =
-                 map (fun p : rpair loc => Locmap.getpair p (call_regs_ext ls1 sg)) (loc_parameters sg)).
-    { admit. (* Same proof *) }
-    destruct (Genv.type_of_call tge (comp_of tf) (Genv.find_comp tge vf)) eqn:TY_CALL.
-    { rewrite R. rewrite <- find_comp_translated.
-      eapply call_trace_lessdef with (ge := ge); eauto using senv_preserved, symbols_preserved. }
+    (* destruct (Genv.type_of_call tge (comp_of tf) (Genv.find_comp tge vf)) eqn:TY_CALL. *)
+    (* { rewrite R. rewrite <- find_comp_translated. *)
+    (*   eapply call_trace_lessdef with (ge := ge); eauto using senv_preserved, symbols_preserved. } *)
     { rewrite R'. rewrite <- find_comp_translated.
       eapply call_trace_lessdef with (ge := ge); eauto using senv_preserved, symbols_preserved. }
-    { rewrite R. rewrite <- find_comp_translated.
-      eapply call_trace_lessdef with (ge := ge); eauto using senv_preserved, symbols_preserved. } }
+    (* { rewrite R. rewrite <- find_comp_translated. *)
+    (*   eapply call_trace_lessdef with (ge := ge); eauto using senv_preserved, symbols_preserved. } *)
+  }
   traceEq. traceEq.
   exploit analyze_successors; eauto. simpl. left; eauto. intros [enext [U V]].
   econstructor; eauto.
@@ -2747,18 +2794,40 @@ Proof.
     unfold Genv.find_comp.
     rewrite H0. now rewrite comp_transf_fundef. }
   rewrite find_comp_translated, SIG.
+  (* destruct (Genv.type_of_call ge (comp_of tf) (Genv.find_comp tge vf)) eqn:TY_CALL. *)
+  (* { *)
+  (* econstructor; eauto. *)
+  (* inv WTI. congruence. *)
+  (* rewrite TY_CALL. *)
+  (* intros. exploit (exec_moves mv2). eauto. eauto. *)
+  (* eapply function_return_satisf with (v := v) (ls_before := ls1) (ls_after := ls0); eauto. *)
+  (* eapply add_equation_ros_satisf; eauto. *)
+  (* eapply add_equations_args_satisf; eauto. *)
+  (* (* rewrite find_comp_translated in R. rewrite <- R in H3. Search tfd. Search fd. *) *)
+  (* (* congruence. *) *)
+  (* (* admit. (* FIXME -- does everything line up later? *) *) *)
+  (* apply wt_regset_assign; auto. *)
+  (* intros [ls2 [A2 B2]]. *)
+  (* exists ls2; split. *)
+  (* eapply star_right. eexact A2. constructor. traceEq. *)
+  (* apply satisf_incr with eafter; auto. *)
+  (* } *)
+  { (* new case *)
   econstructor; eauto.
   inv WTI. congruence.
+  (* rewrite TY_CALL. *)
   intros. exploit (exec_moves mv2). eauto. eauto.
-  eapply function_return_satisf with (v := v) (ls_before := ls1) (ls_after := ls0); eauto.
+  (* no_caller_saves vs _ext *)
+  eapply function_return_satisf_ext with (v := v) (ls_before := ls1) (ls_after := ls0); eauto.
   eapply add_equation_ros_satisf; eauto.
   eapply add_equations_args_satisf; eauto.
-  (* congruence. *)
   apply wt_regset_assign; auto.
   intros [ls2 [A2 B2]].
   exists ls2; split.
   eapply star_right. eexact A2. constructor. traceEq.
   apply satisf_incr with eafter; auto.
+  }
+  (* { } *)
   rewrite SIG. eapply add_equations_args_lessdef; eauto.
   inv WTI. rewrite <- H7. apply wt_regset_list; auto.
   simpl. red; auto.
@@ -2791,7 +2860,7 @@ Proof.
   destruct (transf_function_inv _ _ FUN); auto.
   rewrite SIG'. rewrite return_regs_arg_values; auto. eapply add_equations_args_lessdef; eauto.
   inv WTI. rewrite <- H6. apply wt_regset_list; auto.
-  apply return_regs_agree_callee_save.
+  apply return_regs_agree_callee_save_ext.
   rewrite SIG'. inv WTI. rewrite <- H6. apply wt_regset_list; auto.
 
 (* builtin *)
@@ -2859,12 +2928,12 @@ Proof.
   rewrite <- comp_transf_function; eauto. eauto. eauto. traceEq.
   simpl.
   econstructor; eauto.
-  destruct (Genv.type_of_call tge (call_comp ts) (callee_comp ts)) eqn:TY_CALL;
-    rewrite <- type_of_call_translated in TY_CALL;
-    rewrite TY_CALL.
-  { apply return_regs_agree_callee_save. }
-  { reflexivity. }
-  { apply return_regs_agree_callee_save. }
+  (* destruct (Genv.type_of_call tge (call_comp ts) (callee_comp ts)) eqn:TY_CALL; *)
+  (*   rewrite <- type_of_call_translated in TY_CALL; *)
+  (*   rewrite TY_CALL. *)
+  (* { apply return_regs_agree_callee_save. } *)
+  { apply return_regs_ext_agree_callee_save_ext. }
+  (* { apply return_regs_agree_callee_save. } *)
   constructor.
 + (* with an argument *)
   exploit (exec_moves mv); eauto. intros [ls1 [A1 B1]].
@@ -2873,22 +2942,22 @@ Proof.
   eapply star_right. eexact A1.
   econstructor.
   rewrite <- comp_transf_function; eauto. eauto. eauto. traceEq.
-  destruct (Genv.type_of_call tge (call_comp ts) (callee_comp ts)) eqn:TY_CALL.
-  { (* original proof *)
-  simpl. econstructor; eauto. rewrite <- H11.
-  replace (Locmap.getpair (map_rpair R (loc_result (RTL.fn_sig f)))
-                          (return_regs (parent_locset ts) ls1))
-  with (Locmap.getpair (map_rpair R (loc_result (RTL.fn_sig f))) ls1).
-  eapply add_equations_res_lessdef; eauto.
-  rewrite <- H14. apply WTRS.
-  generalize (loc_result_caller_save (RTL.fn_sig f)).
-  destruct (loc_result (RTL.fn_sig f)); simpl.
-  intros A; rewrite A; auto.
-  intros [A B]; rewrite A, B; auto.
-  rewrite <- type_of_call_translated in TY_CALL. rewrite TY_CALL.
-  apply return_regs_agree_callee_save.
-  rewrite <- H11, <- H14. apply WTRS.
-  }
+  (* destruct (Genv.type_of_call tge (call_comp ts) (callee_comp ts)) eqn:TY_CALL. *)
+  (* { (* original proof *) *)
+  (* simpl. econstructor; eauto. rewrite <- H11. *)
+  (* replace (Locmap.getpair (map_rpair R (loc_result (RTL.fn_sig f))) *)
+  (*                         (return_regs (parent_locset ts) ls1)) *)
+  (* with (Locmap.getpair (map_rpair R (loc_result (RTL.fn_sig f))) ls1). *)
+  (* eapply add_equations_res_lessdef; eauto. *)
+  (* rewrite <- H14. apply WTRS. *)
+  (* generalize (loc_result_caller_save (RTL.fn_sig f)). *)
+  (* destruct (loc_result (RTL.fn_sig f)); simpl. *)
+  (* intros A; rewrite A; auto. *)
+  (* intros [A B]; rewrite A, B; auto. *)
+  (* rewrite <- type_of_call_translated in TY_CALL. rewrite TY_CALL. *)
+  (* apply return_regs_agree_callee_save. *)
+  (* rewrite <- H11, <- H14. apply WTRS. *)
+  (* } *)
   { (* new case *)
   simpl. econstructor; eauto. rewrite <- H11.
   replace (Locmap.getpair (map_rpair R (loc_result (RTL.fn_sig f)))
@@ -2896,15 +2965,17 @@ Proof.
   with (Locmap.getpair (map_rpair R (loc_result (RTL.fn_sig f))) ls1).
   eapply add_equations_res_lessdef; eauto.
   rewrite <- H14. apply WTRS.
-  (* generalize (loc_result_caller_save (RTL.fn_sig f)). *)
-  destruct (loc_result (RTL.fn_sig f)); simpl.
-  admit.
-  admit.
-  rewrite <- type_of_call_translated in TY_CALL. rewrite TY_CALL.
-  reflexivity.
+  assert (SIG: parent_signature ts = fn_sig tf) by admit. rewrite SIG, <- H11.
+  destruct (loc_result (RTL.fn_sig f)) eqn:RES; simpl.
+  { rewrite RES. simpl. destruct (mreg_eq r r). reflexivity. contradiction. }
+  { rewrite RES. simpl.
+    destruct (mreg_eq rhi rhi); [| contradiction].
+    destruct (mreg_eq rlo rlo); [| contradiction].
+    simpl. rewrite orb_true_r. reflexivity. }
+  apply return_regs_ext_agree_callee_save_ext.
   rewrite <- H11, <- H14. apply WTRS.
   }
-  { (* same as Genv.InternalCall *) admit. }
+  (* { (* same as Genv.InternalCall *) admit. } *)
 
 (* internal function *)
 - monadInv FUN. simpl in *.
@@ -2913,22 +2984,22 @@ Proof.
   intros [m'' [U V]].
   assert (WTRS: wt_regset env (init_regs args (fn_params f))).
   { apply wt_init_regs. inv H0. rewrite wt_params. rewrite H9. auto. }
-  destruct (Genv.type_of_call tge (call_comp ts) (comp_of x)) eqn:TY_CALL.
-  { (* original proof *)
-  exploit (exec_moves mv). eauto. eauto.
-    eapply can_undef_satisf; eauto. eapply compat_entry_satisf; eauto.
-    rewrite call_regs_param_values. eexact ARGS.
-    exact WTRS.
-  intros [ls1 [A B]].
-  econstructor; split.
-  eapply plus_left. econstructor; eauto. rewrite <- COMP; eauto.
-  rewrite TY_CALL.
-  eapply star_left. econstructor; eauto.
-  eapply star_right. eexact A.
-  econstructor; eauto.
-  eauto. eauto. traceEq.
-  econstructor; eauto.
-  }
+  (* destruct (Genv.type_of_call tge (call_comp ts) (comp_of x)) eqn:TY_CALL. *)
+  (* { (* original proof *) *)
+  (* exploit (exec_moves mv). eauto. eauto. *)
+  (*   eapply can_undef_satisf; eauto. eapply compat_entry_satisf; eauto. *)
+  (*   rewrite call_regs_param_values. eexact ARGS. *)
+  (*   exact WTRS. *)
+  (* intros [ls1 [A B]]. *)
+  (* econstructor; split. *)
+  (* eapply plus_left. econstructor; eauto. rewrite <- COMP; eauto. *)
+  (* rewrite TY_CALL. *)
+  (* eapply star_left. econstructor; eauto. *)
+  (* eapply star_right. eexact A. *)
+  (* econstructor; eauto. *)
+  (* eauto. eauto. traceEq. *)
+  (* econstructor; eauto. *)
+  (* } *)
   { (* new case *)
   exploit (exec_moves mv). eauto. eauto.
     eapply can_undef_satisf; eauto. eapply compat_entry_satisf; eauto.
@@ -2937,7 +3008,7 @@ Proof.
   intros [ls1 [A B]].
   econstructor; split.
   eapply plus_left. econstructor; eauto. rewrite <- COMP; eauto.
-  rewrite TY_CALL.
+  (* rewrite TY_CALL. *)
   eapply star_left. econstructor; eauto.
   assert (SIG: parent_signature ts = fn_sig x) by admit. rewrite SIG.
   eapply star_right. eexact A.
@@ -2945,7 +3016,7 @@ Proof.
   eauto. eauto. traceEq.
   econstructor; eauto.
   }
-  { (* same as Genv.InternalCall *) admit. }
+  (* { (* same as Genv.InternalCall *) admit. } *)
 
 (* external function *)
 - exploit external_call_mem_extends; eauto. intros [v' [m'' [F [G [J K]]]]].
@@ -2962,28 +3033,53 @@ Proof.
   { rewrite <- B. eapply external_call_well_typed; eauto. }
   rewrite Locmap.gss. rewrite Locmap.gso by (red; auto). rewrite Locmap.gss.
   rewrite val_longofwords_eq_1 by auto. auto.
-  destruct (Genv.type_of_call ge (call_comp ts) (callee_comp ts)) eqn:TY_CALL.
-  {
-  red; intros. rewrite (AG l H0).
-  rewrite locmap_get_set_loc_result_callee_save by auto.
-  unfold undef_caller_save_regs. destruct l; simpl in H0.
-  rewrite H0; auto.
-  destruct sl; auto; congruence.
+  (* destruct (Genv.type_of_call ge (call_comp ts) (callee_comp ts)) eqn:TY_CALL. *)
+  (* { *)
+  (* red; intros. rewrite (AG l H0). *)
+  (* rewrite locmap_get_set_loc_result_callee_save by auto. *)
+  (* unfold undef_caller_save_regs. destruct l; simpl in H0. *)
+  (* rewrite H0; auto. *)
+  (* destruct sl; auto; congruence. *)
+  (* } *)
+  { (* new case *)
+    red; intros.
+    rewrite (AG l H0).
+    rewrite locmap_get_set_loc_result_callee_save_ext by auto.
+    (* rewrite locmap_get_set_loc_result_callee_save by auto. *)
+    unfold undef_caller_save_regs. destruct l; simpl in H0.
+    contradiction.
+    destruct sl; auto; congruence.
   }
-  { (* new case *) reflexivity. }
-  { (* same as Genv.InternalCall *)
-  red; intros. rewrite (AG l H0).
-  rewrite locmap_get_set_loc_result_callee_save by auto.
-  unfold undef_caller_save_regs. destruct l; simpl in H0.
-  rewrite H0; auto.
-  destruct sl; auto; congruence.
-  }
+  (* { (* same as Genv.InternalCall *) *)
+  (* red; intros. rewrite (AG l H0). *)
+  (* rewrite locmap_get_set_loc_result_callee_save by auto. *)
+  (* unfold undef_caller_save_regs. destruct l; simpl in H0. *)
+  (* rewrite H0; auto. *)
+  (* destruct sl; auto; congruence. *)
+  (* } *)
   eapply external_call_well_typed; eauto.
 
 (* return *)
 - inv STACKS.
-  simpl in AG. destruct (Genv.type_of_call ge (comp_of tf) cp) eqn:TY_CALL.
-  {
+  simpl in AG.
+  (* destruct (Genv.type_of_call ge (comp_of tf) cp) eqn:TY_CALL. *)
+  (* { *)
+  (* exploit STEPS; eauto. rewrite WTRES0; auto. intros [ls2 [A B]]. *)
+  (* econstructor; split. *)
+  (* eapply plus_left. constructor. *)
+  (* destruct (transf_function_inv _ _ FUN). *)
+  (* rewrite <- COMP. rewrite <- type_of_call_translated. *)
+  (* intros G. specialize (NO_CROSS_PTR G). clear -SIG RES NO_CROSS_PTR. *)
+  (* unfold loc_result, proj_sig_res in *. rewrite SIG in *. *)
+  (* now inv RES. *)
+  (* destruct (transf_function_inv _ _ FUN). *)
+  (* unfold loc_result, proj_sig_res in *. rewrite SIG in *. *)
+  (* rewrite <- COMP. eapply return_trace_lessdef; eauto using senv_preserved. *)
+  (* eexact A. traceEq. *)
+  (* econstructor; eauto. *)
+  (* apply wt_regset_assign; auto. rewrite WTRES0; auto. *)
+  (* } *)
+  { (* new case, now identical to the others *)
   exploit STEPS; eauto. rewrite WTRES0; auto. intros [ls2 [A B]].
   econstructor; split.
   eapply plus_left. constructor.
@@ -2999,12 +3095,22 @@ Proof.
   econstructor; eauto.
   apply wt_regset_assign; auto. rewrite WTRES0; auto.
   }
-  { (* new case *)
-  rewrite <- (comp_transf_function _ _ FUN) in TY_CALL.
-  apply NO_CROSS_PTR in TY_CALL.
-  (* FIXME *) admit.
-  }
-  { (* same as Genv.InternalCall *) admit. }
+  (* { (* same as Genv.InternalCall *) *)
+  (* exploit STEPS; eauto. rewrite WTRES0; auto. intros [ls2 [A B]]. *)
+  (* econstructor; split. *)
+  (* eapply plus_left. constructor. *)
+  (* destruct (transf_function_inv _ _ FUN). *)
+  (* rewrite <- COMP. rewrite <- type_of_call_translated. *)
+  (* intros G. specialize (NO_CROSS_PTR G). clear -SIG RES NO_CROSS_PTR. *)
+  (* unfold loc_result, proj_sig_res in *. rewrite SIG in *. *)
+  (* now inv RES. *)
+  (* destruct (transf_function_inv _ _ FUN). *)
+  (* unfold loc_result, proj_sig_res in *. rewrite SIG in *. *)
+  (* rewrite <- COMP. eapply return_trace_lessdef; eauto using senv_preserved. *)
+  (* eexact A. traceEq. *)
+  (* econstructor; eauto. *)
+  (* apply wt_regset_assign; auto. rewrite WTRES0; auto. *)
+  (* } *)
 (* Qed. *)
 Admitted.
 
